src/Zulib/fstar/Zen.ContractResult.NoMessage.fst
@@ -5,22 +5,22 @@ open Zen.Types
 open Zen.Cost
 
 module CR = Zen.ContractResult
-module ET = Zen.ErrorT
+module RT = Zen.ResultT
 
 type t = CR.t
 
 val ofResult: result txSkeleton -> CR.t `cost` 0
 let ofResult =
     function
-    | OK txSkeleton -> ET.ret (txSkeleton,None)
-    | EX e -> ET.autoFail e
-    | ERR msg -> ET.autoFailw msg
+    | OK txSkeleton -> RT.ok (txSkeleton,None)
+    | EX e -> RT.autoFail e
+    | ERR msg -> RT.autoFailw msg
 
 val ofOption: string -> option txSkeleton -> CR.t `cost` 0
 let ofOption msg =
     function
-    | Some txSkeleton -> ET.ret (txSkeleton,None)
-    | None -> ET.failw msg
+    | Some txSkeleton -> RT.ok (txSkeleton,None)
+    | None -> RT.failw msg
 
 val ret: txSkeleton -> CR.t `cost` 0
-let ret txSkeleton = ET.ret (txSkeleton,None)
+let ret txSkeleton = RT.ok (txSkeleton,None)
